Define How Coordinates Define Equivalences (#41)
Closes #28, #49 (HML_SRBB def to handle tau properly) and #51 (document formatting issues)

* defining expressiveness preorder and equivalence
* copy definitions for weak trace preoreder and state lemma to be proven
* move weak trace related lemmas into its own file
* adding proof attempt linking weak step sequence to tradce formulas
* defined weak trace equivalence
* lemma trace_formula_implies_trace
* simplified lemma
* lemma silent_reachable_trans, progress in trace_formula_implies_trace
* trace_formula_implies_trace inductioncase internal
* ugly proof for trace_formula_implies_trace
* progress in lemma t ∈ weak_traces p = ((wtrace_to_φ t) ⊨SRBB p)
* proved lemma (p ≲WT q) = (p ≼ (E ∞ 0 0 0 0 0 0 0) q)
* simplified (p ≲WT q) = (p ≼ (E ∞ 0 0 0 0 0 0 0) q)
* trace_equals_trace_to_formula (but really ugly)
* restructured hml_srbb; lemma trace_equals_trace_to_formula for the new hml_srbb
* lemma aux
* fixed sectioning in Expressiveness_Price.thy
* removed unnecessary stuff
* equi characterizes lemma
* improving readability of auxillary lemma
* removing trivial cases of trace_formula_implies_trace
* fixing bugs due to changed |= argument order
* include weak trace proofs in the build
* removing useless function and lemma

---------

Co-authored-by: ikarus <leonard.moritz.huebner@campus.tu-berlin.de>
Co-authored-by: ekeln <karl.mattes36@gmail.com>

HML_SRBB.thy
@@ -31,7 +31,8 @@ primrec
   "hml_srbb_to_hml (Internal \<chi>) = hml.Internal (hml_srbb_conjunction_to_hml \<chi>)" |
   "hml_srbb_to_hml (ImmConj I \<psi>s) = hml.Conj I (hml_srbb_conjunct_to_hml_conjunct \<circ> \<psi>s)" |
 
-  "hml_srbb_conjunction_to_hml (Obs a \<phi>) = hml.Obs a (hml_srbb_to_hml \<phi>)" |
+  "hml_srbb_conjunction_to_hml (Obs a \<phi>) = HML_soft_poss a (hml_srbb_to_hml \<phi>)" |
+(*equivalent to? (if a = \<tau> then hml_srbb_to_hml \<phi> else hml.Obs a (hml_srbb_to_hml \<phi>))*)
   "hml_srbb_conjunction_to_hml (Conj I \<psi>s) = hml.Conj I (hml_srbb_conjunct_to_hml_conjunct \<circ> \<psi>s)" |
 
   "hml_srbb_conjunction_to_hml (StableConj I \<psi>s) =
@@ -47,6 +48,9 @@ primrec
 
 fun hml_srbb_models :: "'s \<Rightarrow> ('a, 's) hml_srbb \<Rightarrow> bool" (infix "\<Turnstile>SRBB" 60)where
   "hml_srbb_models state formula = (state \<Turnstile> (hml_srbb_to_hml formula))"
+
+fun hml_srbb_conjunction_models :: "('a, 's) hml_srbb_conjunction \<Rightarrow> 's \<Rightarrow> bool" where
+  "hml_srbb_conjunction_models \<chi> s = (s \<Turnstile> (hml_srbb_conjunction_to_hml \<chi>))"
 
 (*Some sanity checks*)
 
