Weak_Traces.thy
@@ -1,0 +1,307 @@
+theory Weak_Traces
+  imports Main HML_SRBB Expressiveness_Price
+begin
+
+inductive
+      is_trace_formula :: "('act, 'i) hml_srbb \<Rightarrow> bool"
+  and is_trace_formula_conjunction :: "('act, 'i) hml_srbb_conjunction \<Rightarrow> bool" where
+  "is_trace_formula TT" |
+  "is_trace_formula (Internal \<chi>)" if "is_trace_formula_conjunction \<chi>" |
+  "is_trace_formula_conjunction (Obs \<alpha> \<phi>)" if "is_trace_formula \<phi>"
+
+
+fun wtrace_to_\<phi> :: "'act list \<Rightarrow> ('act, 'i) hml_srbb"
+  and wtrace_to_\<chi> :: "'act list \<Rightarrow> ('act, 'i) hml_srbb_conjunction"
+  and wtrace_to_\<psi> :: "'act list \<Rightarrow> ('act, 'i) hml_srbb_conjunct" where
+  "wtrace_to_\<phi> [] = TT" |
+  "wtrace_to_\<phi> tr = (Internal (wtrace_to_\<chi> tr))" |
+
+  "wtrace_to_\<chi> [] = (Conj {} (\<lambda>_. undefined))" | \<comment> \<open> Should never happen\<close>
+  "wtrace_to_\<chi> (\<alpha> # tr) = (Obs \<alpha> (wtrace_to_\<phi> tr))" |
+
+  "wtrace_to_\<psi> tr = Pos (wtrace_to_\<chi> tr)" \<comment> \<open>Should never happen\<close>
+
+lemma trace_to_\<phi>_is_trace_formula:
+  "is_trace_formula (wtrace_to_\<phi> trace)"
+  apply (induct trace)
+  using is_trace_formula_is_trace_formula_conjunction.intros
+  by fastforce+
+
+lemma trace_formula_to_expressiveness:
+  fixes \<phi> :: "('act, 'i) hml_srbb"
+  fixes \<chi> :: "('act, 'i) hml_srbb_conjunction"
+  shows  "(is_trace_formula \<phi>             \<longrightarrow> (\<phi> \<in> \<O> (E \<infinity> 0 0 0 0 0 0 0)))
+        \<and> (is_trace_formula_conjunction \<chi> \<longrightarrow> (\<chi> \<in> \<O>_\<chi> (E \<infinity> 0 0 0 0 0 0 0)))"
+  apply (rule is_trace_formula_is_trace_formula_conjunction.induct)
+  by (simp add: \<O>_def \<O>_\<chi>_def leq_not_eneg)+
+
+lemma expressiveness_to_trace_formula:
+  fixes \<phi> :: "('act, 'i) hml_srbb"
+  fixes \<chi> :: "('act, 'i) hml_srbb_conjunction"
+  shows "(\<phi> \<in> \<O> (E \<infinity> 0 0 0 0 0 0 0) \<longrightarrow> is_trace_formula \<phi>)
+       \<and> (\<chi> \<in> \<O>_\<chi> (E \<infinity> 0 0 0 0 0 0 0) \<longrightarrow> is_trace_formula_conjunction \<chi>) 
+       \<and> True"
+  apply (rule hml_srbb_hml_srbb_conjunction_hml_srbb_conjunct.induct)
+  using is_trace_formula_is_trace_formula_conjunction.intros(1) apply blast
+  apply (simp add: \<O>_\<chi>_def \<O>_def is_trace_formula_is_trace_formula_conjunction.intros(2))
+  apply (simp add: \<O>_def leq_not_eneg)
+  by (simp add: \<O>_\<chi>_def \<O>_def is_trace_formula_is_trace_formula_conjunction.intros(3) leq_not_eneg)+
+
+lemma modal_depth_only_is_trace_form: 
+  "(is_trace_formula \<phi>) = (\<phi> \<in> \<O> (E \<infinity> 0 0 0 0 0 0 0))"
+  using expressiveness_to_trace_formula trace_formula_to_expressiveness by blast
+
+context Inhabited_Tau_LTS
+begin                 
+
+lemma trace_formula_implies_trace:
+  fixes \<psi> ::"('a, 's) hml_srbb_conjunct"
+  shows
+       trace_case: "is_trace_formula \<phi> \<Longrightarrow> p \<Turnstile>SRBB \<phi> \<Longrightarrow> (\<exists>tr \<in> weak_traces p. wtrace_to_\<phi> tr = \<phi>)"
+    and conj_case: "is_trace_formula_conjunction \<chi> \<Longrightarrow> hml_srbb_conjunction_models \<chi> q \<Longrightarrow> (\<exists>tr \<in> weak_traces q. wtrace_to_\<chi> tr = \<chi>)"
+    and            True
+  apply (induction \<phi> and \<chi> and \<psi> arbitrary: p and q)
+  using weak_step_sequence.intros(1) apply fastforce
+  prefer 2 using is_trace_formula.cases apply blast
+  prefer 3 prefer 4 prefer 6 prefer 7
+  using is_trace_formula_conjunction.cases apply blast+
+  prefer 3 apply (simp add: is_trace_formula_conjunction.simps)
+proof-
+  case (Internal \<chi>r)
+  assume IH: "(\<And>q. is_trace_formula_conjunction \<chi>r \<Longrightarrow>
+                 hml_srbb_conjunction_models \<chi>r q \<Longrightarrow> \<exists>tr\<in>weak_traces q. wtrace_to_\<chi> tr = \<chi>r)"
+and is_trace_internal :"is_trace_formula (hml_srbb.Internal \<chi>r)"
+and internal_satisfied: "p \<Turnstile>SRBB hml_srbb.Internal \<chi>r"
+  from Internal(3) obtain p' where wtrace_to_p': "p \<Zsurj> p'" and p'_models_\<chi>r: "hml_srbb_conjunction_models \<chi>r p'" 
+    by auto
+  from Internal(2) have "is_trace_formula_conjunction \<chi>r"
+    using is_trace_formula.cases by auto
+  with p'_models_\<chi>r IH obtain tail p'' where tail_in_traces_p': "tail \<in> weak_traces p'" "wtrace_to_\<chi> tail = \<chi>r" "p' \<Zsurj>\<mapsto>\<Zsurj>$ tail p''"
+    by blast
+  then show ?case
+  proof(cases tail)
+    case Nil
+    hence False
+      using \<open>is_trace_formula_conjunction \<chi>r\<close> is_trace_formula_conjunction.simps tail_in_traces_p'(2) by force
+    then show ?thesis by blast
+  next
+    case (Cons a list)
+    then obtain q' where q'_properties:"p' \<Zsurj>\<mapsto>\<Zsurj> a q' \<and> q' \<Zsurj>\<mapsto>\<Zsurj>$ list p''"
+      using \<open>p' \<Zsurj>\<mapsto>\<Zsurj>$ tail p''\<close> weak_step_sequence.cases 
+      by (metis list.discI list.inject)
+    hence "p \<Zsurj>\<mapsto>\<Zsurj> a q'" using wtrace_to_p' silent_reachable_trans weak_step_def
+      by metis
+    with q'_properties have "p \<Zsurj>\<mapsto>\<Zsurj>$ tail p''" 
+      using Cons weak_step_sequence.intros(2) by blast
+    then show ?thesis
+      using Cons tail_in_traces_p'(2) by auto 
+  qed
+next
+  case (Obs \<alpha> \<phi>r)
+  assume IH: "(\<And>p. is_trace_formula \<phi>r \<Longrightarrow> p \<Turnstile>SRBB \<phi>r \<Longrightarrow> \<exists>tr\<in>weak_traces p. wtrace_to_\<phi> tr = \<phi>r)"
+and obs_is_trace:"is_trace_formula_conjunction (hml_srbb_conjunction.Obs \<alpha> \<phi>r)"
+and obs_models_q: "hml_srbb_conjunction_models (hml_srbb_conjunction.Obs \<alpha> \<phi>r) q"
+  from obs_is_trace have \<phi>r_is_trace: "is_trace_formula \<phi>r"
+    using is_trace_formula_conjunction.cases by auto
+  from obs_models_q have hml_models: "q \<Turnstile> hml_srbb_conjunction_to_hml (Obs \<alpha> \<phi>r)"
+    by simp
+  then show ?case
+  proof(cases \<open>\<alpha> = \<tau>\<close>)
+    case True
+    with hml_models have "q \<Turnstile> hml.Silent (hml_srbb_to_hml \<phi>r)" 
+      using hml_srbb_conjunction_to_hml.simps 
+      by force
+    then obtain q' where "(q \<mapsto> \<tau> q' \<and> (q' \<Turnstile>SRBB \<phi>r)) \<or> (q \<Turnstile>SRBB \<phi>r)"
+      using hml_models.simps(4)
+      by fastforce
+    then show ?thesis 
+    proof
+      assume assm: "q \<mapsto> \<tau> q' \<and> q' \<Turnstile>SRBB \<phi>r"
+      with IH \<phi>r_is_trace  obtain tail where "tail\<in>weak_traces q'" "wtrace_to_\<phi> tail = \<phi>r"
+        by blast
+      with assm show ?thesis
+        using LTS_Tau.weak_step_sequence.intros(2) True silent_reachable.intros weak_step_def 
+        by fastforce
+    next
+      assume "q \<Turnstile>SRBB \<phi>r"
+      with IH \<phi>r_is_trace show ?thesis 
+        using LTS_Tau.weak_step_sequence.intros(2) True silent_reachable.intros(1) weak_step_def 
+        by fastforce
+    qed
+  next
+    case False
+    hence "q \<Turnstile> hml.Obs \<alpha> (hml_srbb_to_hml \<phi>r)" 
+      using hml_srbb_conjunction_to_hml.simps hml_models by presburger
+    then obtain q' where \<alpha>_step: "q \<mapsto> \<alpha> q'" and \<phi>r_models_q': "q' \<Turnstile>SRBB \<phi>r"
+      by auto
+    with IH \<phi>r_is_trace obtain tail where tail_in_wt_q': "tail \<in>weak_traces q'" "wtrace_to_\<phi> tail = \<phi>r"
+      by blast
+    from \<alpha>_step have "q \<Zsurj>\<mapsto>\<Zsurj> \<alpha> q'" 
+      unfolding weak_step_def using silent_reachable.simps by metis
+    hence wt_q_to_q': "q \<Zsurj>\<mapsto>\<Zsurj>$ [\<alpha>] q'" 
+      using weak_step_sequence.simps unfolding weak_step_def using silent_reachable.simps
+      by (smt (verit, best))
+    with tail_in_wt_q' have "(\<alpha>#tail) \<in> weak_traces q" using weak_step_sequence_trans
+      by fastforce
+    then show ?thesis 
+      using tail_in_wt_q'(2) by fastforce
+  qed
+qed
+
+lemma trace_equals_trace_to_formula: 
+  "t \<in> weak_traces p = (p \<Turnstile>SRBB (wtrace_to_\<phi> t))"
+proof
+  assume "t \<in> weak_traces p"
+  show "p \<Turnstile>SRBB (wtrace_to_\<phi> t)"
+    using \<open>t \<in> weak_traces p\<close>
+  proof(induction t arbitrary: p)
+    case Nil
+    then show ?case 
+      by simp
+  next
+    case (Cons a tail)
+    from Cons obtain p'' p' where "p \<Zsurj>\<mapsto>\<Zsurj> a p''" "p'' \<Zsurj>\<mapsto>\<Zsurj>$ tail p'" using weak_step_sequence.simps 
+      by (smt (verit, best) list.discI list.inject mem_Collect_eq) 
+    with Cons(1) have IS: "p'' \<Turnstile>SRBB wtrace_to_\<phi> tail"
+      by blast
+    hence IS_2: "p'' \<Turnstile> (hml_srbb_to_hml (wtrace_to_\<phi> tail))" by simp
+    from Cons have goal_eq: "wtrace_to_\<phi> (a # tail) = (Internal (Obs a (wtrace_to_\<phi> tail)))"
+      by simp
+    show ?case
+    proof(cases \<open>a = \<tau>\<close>)
+      case True
+      with goal_eq have "p \<Turnstile>SRBB (wtrace_to_\<phi> (a # tail)) = 
+(p \<Turnstile> hml.Internal (hml.Silent (hml_srbb_to_hml (wtrace_to_\<phi> tail))))"
+        by force
+      also have "... = 
+(\<exists>p'. p \<Zsurj> p' \<and> (((\<exists>p''. p' \<mapsto> \<tau> p'' \<and> (p'' \<Turnstile> (hml_srbb_to_hml (wtrace_to_\<phi> tail)))) \<or> 
+(p' \<Turnstile> (hml_srbb_to_hml (wtrace_to_\<phi> tail))))))"
+        by force
+      with \<open>p \<Zsurj>\<mapsto>\<Zsurj> a p''\<close> True IS_2 show ?thesis 
+        using weak_step_def by auto
+    next
+      case False
+      hence "wtrace_to_\<phi> (a#tail) = 
+(Internal (Obs a (wtrace_to_\<phi> tail)))"
+        by simp
+      hence converted_srbb_sat:  "(p \<Turnstile>SRBB wtrace_to_\<phi> (a # tail)) =
+(\<exists>p'. p \<Zsurj> p' \<and> ((\<exists>p''. p' \<mapsto> a p'' \<and> p'' \<Turnstile>SRBB wtrace_to_\<phi> tail)))"
+        by (simp add: False)
+      with IS_2 False \<open>p \<Zsurj>\<mapsto>\<Zsurj> a p''\<close> show ?thesis 
+        by (smt (verit, best) LTS_Tau.hml_models.simps(1) LTS_Tau.hml_models.simps(3) 
+LTS_Tau.silent_reachable_trans hml_srbb_models.elims(3) hml_srbb_to_hml.simps(1) 
+hml_srbb_to_hml.simps(2) weak_step_def wtrace_to_\<phi>.elims) 
+    qed
+  qed
+next
+  assume "p \<Turnstile>SRBB wtrace_to_\<phi> t"
+  then show "t \<in> weak_traces p"
+  proof(induction t arbitrary: p)
+    case Nil
+    then show ?case
+      using weak_step_sequence.intros(1) by fastforce
+  next
+    case (Cons a tail)
+    hence "p \<Turnstile>SRBB (Internal (Obs a (wtrace_to_\<phi> tail)))"
+      by simp
+    hence 1: "p \<Turnstile> (hml_srbb_to_hml (Internal (Obs a (wtrace_to_\<phi> tail))))"
+      by simp
+    show ?case
+      proof(cases \<open>a = \<tau>\<close>)
+        case True
+        with 1 have "p \<Turnstile> (hml.Internal (hml.Silent (hml_srbb_to_hml (wtrace_to_\<phi> tail))))"
+          by simp
+        then obtain p' p'' where "(p \<Zsurj> p' \<and> (p' \<mapsto> \<tau> p'' \<and> 
+(p'' \<Turnstile> (hml_srbb_to_hml (wtrace_to_\<phi> tail)))) \<or> 
+(p \<Zsurj> p' \<and> (p' \<Turnstile> (hml_srbb_to_hml (wtrace_to_\<phi> tail)))))" 
+          by fastforce
+        then show ?thesis
+        proof
+          assume assms: "(p \<Zsurj> p') \<and> p' \<mapsto> \<tau> p'' \<and> (p'' \<Turnstile> hml_srbb_to_hml (wtrace_to_\<phi> tail))"
+          with Cons have "tail \<in> weak_traces p''"
+            using hml_srbb_models.simps by blast
+          from assms have "p \<Zsurj>\<mapsto>\<Zsurj> \<tau> p''" 
+            using weak_step_def LTS_Tau.silent_reachable_trans silent_reachable.intros 
+            by metis
+          with True \<open>tail \<in> weak_traces p''\<close> show ?thesis 
+            using weak_step_sequence.intros(2) by fastforce
+        next
+          assume assms: "p \<Zsurj> p' \<and> (p' \<Turnstile> hml_srbb_to_hml (wtrace_to_\<phi> tail))"
+          show "a # tail \<in> weak_traces p"
+          proof-
+            from assms Cons have "tail \<in> weak_traces p'" 
+              by auto
+            from assms have "p \<Zsurj>\<mapsto>\<Zsurj> \<tau> p'"
+              using weak_step_def by fastforce
+            with \<open>tail \<in> weak_traces p'\<close> have "(\<tau> # tail) \<in> weak_traces p" 
+              using weak_step_sequence.intros(2) by fastforce
+            with True show "a # tail \<in> weak_traces p" by simp
+          qed
+        qed
+      next
+        case False
+        with Cons(2) have "p \<Turnstile>SRBB wtrace_to_\<phi> ((a # tail))"
+        by auto
+      hence restructure: "p \<Turnstile>SRBB (Internal (Obs a (wtrace_to_\<phi> tail)))" 
+        by force
+      have "(p \<Turnstile>SRBB (wtrace_to_\<phi> tail))= 
+(p \<Turnstile> (hml_srbb_to_hml (wtrace_to_\<phi> tail)))"
+        by simp
+        with Cons(2) restructure obtain p' p'' where 
+"p \<Zsurj> p'" "p' \<mapsto> a p''" "p'' \<Turnstile> ((hml_srbb_to_hml (wtrace_to_\<phi> tail)))" 
+          using False by auto
+from this(1, 2) have "p \<Zsurj>\<mapsto>\<Zsurj> a p''" unfolding weak_step_def using silent_reachable.intros 
+      by (metis silent_reachable_trans)
+    from \<open>p'' \<Turnstile> ((hml_srbb_to_hml (wtrace_to_\<phi> tail)))\<close> 
+    have "p'' \<Turnstile>SRBB wtrace_to_\<phi> tail"
+      by simp
+    with \<open>p \<Zsurj>\<mapsto>\<Zsurj> a p''\<close> show "(a#tail) \<in> weak_traces p" 
+      using weak_step_sequence.intros(2) 
+      using Cons.IH by fastforce
+  qed
+qed
+qed
+
+lemma aux:
+  fixes \<phi> :: "('a, 's) hml_srbb"
+  fixes \<chi> :: "('a, 's) hml_srbb_conjunction"
+  fixes \<psi> :: "('a, 's) hml_srbb_conjunct"
+  shows "p \<lesssim>WT q \<Longrightarrow> is_trace_formula \<phi> \<Longrightarrow> p \<Turnstile>SRBB \<phi> \<Longrightarrow> q \<Turnstile>SRBB \<phi>"
+proof -
+  assume \<phi>_trace: "is_trace_formula \<phi>" and p_sat_\<phi>: "p \<Turnstile>SRBB \<phi>" and assms: "p \<lesssim>WT q"
+  show "q \<Turnstile>SRBB \<phi>"
+  proof-
+    from assms have p_trace_implies_q_trace: "\<forall>tr p'. (p \<Zsurj>\<mapsto>\<Zsurj>$ tr p') \<longrightarrow> (\<exists>q'. q \<Zsurj>\<mapsto>\<Zsurj>$ tr q')" 
+      unfolding weakly_trace_preordered_def by auto
+    from p_sat_\<phi> trace_formula_implies_trace obtain tr p' where 
+      "(p \<Zsurj>\<mapsto>\<Zsurj>$ tr p')" "wtrace_to_\<phi> tr = \<phi>"
+      using \<phi>_trace by blast
+    with p_trace_implies_q_trace obtain q' where "q \<Zsurj>\<mapsto>\<Zsurj>$ tr q'" 
+      by blast
+    with trace_equals_trace_to_formula show ?thesis 
+      using \<open>wtrace_to_\<phi> tr = \<phi>\<close> by blast
+  qed
+qed
+
+lemma expr_preorder_characterizes_relational_preorder_traces: "(p \<lesssim>WT q) = (p \<preceq> (E \<infinity> 0 0 0 0 0 0 0) q)"
+  unfolding expr_preord_def hml_preordered_def
+proof
+  assume "p \<lesssim>WT q"
+  then show "\<forall>\<phi>\<in>\<O> (E \<infinity> 0 0 0 0 0 0 0). p \<Turnstile>SRBB \<phi> \<longrightarrow> q \<Turnstile>SRBB \<phi>"
+    using aux expressiveness_to_trace_formula weakly_trace_preordered_def
+    by blast+
+next
+  assume \<phi>_eneg: "\<forall>\<phi>\<in>\<O> (E \<infinity> 0 0 0 0 0 0 0). p \<Turnstile>SRBB \<phi> \<longrightarrow> q \<Turnstile>SRBB \<phi>"
+  show "p \<lesssim>WT q"
+    unfolding weakly_trace_preordered_def
+    using \<phi>_eneg trace_equals_trace_to_formula trace_formula_to_expressiveness trace_to_\<phi>_is_trace_formula
+    by (simp, blast+)
+qed
+
+lemma "(p \<simeq>WT q) = (p \<sim> (E \<infinity> 0 0 0 0 0 0 0) q)"
+  unfolding weakly_trace_equivalent_def expr_equiv_def \<O>_def hml_equivalent_def hml_preordered_def
+  using expr_preorder_characterizes_relational_preorder_traces
+  by (simp add: \<O>_def expr_preord_def hml_preordered_def) 
+end
+
+end
